Coq/src/HigherOrder/Effect.v
@@ -1,72 +1,73 @@
-Require Import Thesis.Base.
-Require Import Thesis.Prog.
-Require Import Thesis.Classes.
+Require Import Thesis.HigherOrder.Base.
+Require Import Thesis.HigherOrder.Prog.
+Require Import Thesis.HigherOrder.Classes.
 
 Set Implicit Arguments.
 
 Definition Get : Prog (nat * nat) :=
   let s : @Shape _ NDShare := inl (sget (nat * nat))
-  in impure (ext s (fun p : @Pos _ NDShare s => match p with pget s => pure s end)).
+  in impure (ext s (fun p : @Pos _ NDShare s => match p with pget s => pure s end)
+                 (fun p : @PosX _ NDShare s => match p with end)).
 
 Definition Put (n : nat * nat) : Prog unit :=
   let s : @Shape _ NDShare := inl (sput n)
-  in impure (ext s (fun p : @Pos _ NDShare s => match p with pput s => pure tt end)).
+  in impure (ext s (fun p : @Pos _ NDShare s => match p with pput s => pure tt end)
+                 (fun p : @PosX _ NDShare s => match p with end)).
 
-Definition BeginShare (n : nat * nat) : Prog unit :=
-  let s : @Shape _ NDShare := inr (inl (sbsharing n))
-  in impure (ext s (fun p : @Pos _ NDShare s => pure tt)).
+Definition Share' (n : nat * nat) A (fs : Prog A) : Prog A :=
+  let s : @Shape _ NDShare := inr (inl (ssharing n A))
+  in impure (ext s (fun p : @Pos _ NDShare s => match p with pcont _ s => pure s end)
+                 (fun p : @PosX _ NDShare s => match p with pshared _ => fs end)).
 
-Definition EndShare (n : nat * nat) : Prog unit :=
-  let s : @Shape _ NDShare := inr (inl (sesharing n))
-  in impure (ext s (fun p : @Pos _ NDShare s => pure tt)).
-
-Definition BeginShare__SC A (n : nat * nat) (fp : Prog__SC A) : Prog__SC A :=
-  let s : @Shape _ NDShare__SC := inl (sbsharing n)
-  in impure (ext s (fun p : @Pos _ NDShare__SC s => fp)).
-
-Definition EndShare__SC A (n : nat * nat) (fp : Prog__SC A) : Prog__SC A :=
-  let s : @Shape _ NDShare__SC := inl (sesharing n)
-  in impure (ext s (fun p : @Pos _ NDShare__SC s => fp)).
+Definition Share'__SC (n : nat * nat) A (fs : Prog__SC A) : Prog__SC A :=
+  let s : @Shape _ NDShare__SC := (inl (ssharing n A))
+  in impure (ext s (fun p : @Pos _ NDShare__SC s => match p with pcont _ x => pure x end)
+                 (fun p : @PosX _ NDShare__SC s => match p with pshared _ => fs end)).
 
 Definition Share A `(Shareable A) (fp : Prog A) : Prog (Prog A) :=
   Get >>= fun '(i,j) =>
   Put (i + 1, j) >>= fun _ =>
-  pure (BeginShare (i,j) >>= fun _ =>
-        Put (i, j + 1) >>= fun _ =>
-        fp >>= fun x =>
-        shareArgs x >>= fun x' =>
-        EndShare (i,j) >>= fun _ =>
-        pure x').
+  pure (Share' (i,j)
+               (Put (i, j + 1) >>= fun _ =>
+                fp >>= fun x =>
+                shareArgs x)).
+
 Arguments Share {_} {_} fp.
 
 Definition Fail A : Prog A :=
   let s : @Shape _ NDShare := inr (inr sfail)
-    in impure (ext s (fun p : @Pos _ NDShare s => match p with end)).
+  in impure (ext s (fun p : @Pos _ NDShare s => match p with end)
+                 (fun p : @PosX _ NDShare s => match p with end)).
 
 Arguments Fail {_}.
 
 Definition Fail__C A : Free C__Choice A :=
   let s : @Shape _ C__Choice := sfail
-  in impure (ext s (fun p : Pos__Choice s => match p with end)).
+  in impure (ext s (fun p : Pos__Choice s => match p with end)
+                 (fun p : PosX__Choice s => match p with end)).
 
 Arguments Fail__C {_}.
 
 Definition Fail__SC A : Free (C__Comb C__Sharing C__Choice) A :=
   let s : @Shape _ NDShare__SC := inr sfail
-  in impure (ext s (fun p : @Pos _ NDShare__SC s => match p with end)).
+  in impure (ext s (fun p : @Pos _ NDShare__SC s => match p with end)
+                 (fun p : @PosX _ NDShare__SC s => match p with end)).
 
 Arguments Fail__SC {_}.
 
 Definition Choice__C A mid l r : Free C__Choice A :=
   let s : @Shape _ C__Choice := schoice mid
-  in impure (ext s (fun p : Pos__Choice s => if p then l else r)).
+  in impure (ext s (fun p : Pos__Choice s => if p then l else r)
+                 (fun p : PosX__Choice s => match p with end)).
 
 Definition Choice__SC A mid l r : Prog__SC A :=
   let s : @Shape _ NDShare__SC := inr (schoice mid)
-  in impure (ext s (fun p : @Pos _ NDShare__SC s => if p then l else r)).
+  in impure (ext s (fun p : @Pos _ NDShare__SC s => if p then l else r)
+                 (fun p : @PosX _ NDShare__SC s => match p with end)).
 
 Definition Choice A mid l r : Prog A :=
   let s : @Shape _ NDShare := inr (inr (schoice mid))
-  in impure (ext s (fun p : @Pos _ NDShare s => if p then l else r)).
+  in impure (ext s (fun p : @Pos _ NDShare s => if p then l else r)
+                 (fun p : @PosX _ NDShare s => match p with end)).
 
 Notation "x ? y" := (Choice None x y) (at level 80).
