Coq/src/HigherOrder/Classes.v
@@ -1,0 +1,14 @@
+Require Import Thesis.HigherOrder.Prog.
+
+Class Shareable (A : Type) :=
+  {
+    shareArgs : A -> Prog A
+  }.
+
+Class Normalform (A B : Type) :=
+  {
+    nf : Prog A -> Prog B;
+    nf_impure: forall s (pf : _ -> Prog A) pfx,
+        nf (impure (ext s pf pfx)) = impure (ext s (fun p => nf (pf p)) pfx)
+
+  }.
