Coq/src/HigherOrder/DataM.v
@@ -1,0 +1,231 @@
+Require Import Thesis.HigherOrder.Prog.
+Require Import Thesis.HigherOrder.Base.
+Require Import Thesis.HigherOrder.Effect.
+Require Import Thesis.HigherOrder.Classes.
+Require Import Thesis.HigherOrder.Handler.
+
+Set Implicit Arguments.
+
+Section Prim.
+  Definition Coin : Prog nat := Choice None (pure 0) (pure 1).
+  Definition Coin__Bool : Prog bool := Choice None (pure true) (pure false).
+  
+  Definition addM (fn1 fn2 : Prog nat) : Prog nat :=
+    fn1 >>= fun n1 => fn2 >>= fun n2 => pure (n1 + n2).
+  
+  Definition orM (fn1 fn2 : Prog bool) : Prog bool :=
+    fn1 >>= fun b => match b with
+                  | true => pure true
+                  | false => fn2
+                  end.
+  
+  Definition notM (fn : Prog bool) : Prog bool :=
+    fn >>= fun b => pure (negb b).
+ 
+  Definition duplicate A (fx : Prog A) : Prog (A * A) :=
+    fx >>= fun x => fx >>= fun y => pure (x,y).
+
+  Global Instance shareable__Nat : Shareable nat :=
+    {
+      shareArgs := pure
+    }.
+  
+  Global Instance shareable__Bool : Shareable bool :=
+    {
+      shareArgs := pure
+    }.
+
+  Definition nf__nat (n : Prog nat) :=
+    free_bind n (fun n' => pure n').
+
+  Lemma nf_impure__nat : forall s (pf : _ -> Prog nat),
+      nf__nat (impure (ext s pf)) = impure (ext s (fun p => nf__nat (pf p))).
+  Proof. trivial. Qed.
+
+  Global Instance normalform__nat : Normalform nat nat :=
+    {
+      nf := nf__nat;
+      nf_impure := nf_impure__nat
+    }.
+  
+  Definition nf__bool (b : Prog bool) :=
+    b >>= fun b' => pure b'.
+
+  Lemma nf_impure__bool : forall s (pf : _ -> Prog bool),
+      nf__bool (impure (ext s pf)) = impure (ext s (fun p => nf__bool (pf p))).
+  Proof. trivial. Qed.
+
+  Global Instance normalform__bool : Normalform bool bool :=
+    {
+      nf := nf__bool;
+      nf_impure := nf_impure__bool
+    }.
+End Prim.
+
+Section Pair.
+  Inductive Pair A B :=
+  | Pair' : Prog A -> Prog B -> Pair A B.
+  
+  Definition pairM A B (fst : Prog A) (snd : Prog B) : Prog (Pair A B) :=
+    pure (Pair' fst snd).
+
+  Definition firstM A B (fp : Prog (Pair A B)) : Prog A :=
+    fp >>= fun '(Pair' fst _) => fst.
+
+  Definition secondM A B (fp : Prog (Pair A B)) : Prog B :=
+    fp >>= fun '(Pair' _ snd) => snd.
+
+  Definition dup' (fp : Prog (Pair bool bool)) : Prog (Pair bool bool) :=
+    pairM (firstM fp) (firstM fp).
+
+  Definition dup A (fx : Prog A) : Prog (Pair A A) :=
+    pairM fx fx.
+
+  Definition dupShare A `{Shareable A} (fx : Prog A) : Prog (Pair A A) :=
+    Share fx >>= fun x => pairM x x.
+
+  Definition shareArgs__Pair A B `(Shareable A) `(Shareable B) (p : Pair A B) : Prog (Pair A B) :=
+    match p with
+    | Pair' a b => Share a >>= fun sa => Share b >>= fun sb => pairM sa sb
+    end.
+
+  Global Instance shareable__Pair A B `(sa : Shareable A) `(sb : Shareable B) : Shareable (Pair A B) :=
+    {
+      shareArgs := @shareArgs__Pair A B sa sb
+    }.
+
+  Definition nf__Pair A B C D `{Normalform A C} `{Normalform B D} (stp : Prog (Pair A B)) : Prog (Pair C D) :=
+    stp >>= fun '(Pair' sp1 sp2) =>
+              nf sp1 >>= fun b1 =>
+                           nf sp2 >>= fun b2 =>
+                                        pairM (pure b1) (pure b2).
+
+  Lemma nf_impure__Pair A B C D nf__AC nf__BD : forall s (pf : _ -> Prog (Pair A B)),
+      @nf__Pair A B C D nf__AC nf__BD (impure (ext s pf)) = impure (ext s (fun p => nf__Pair (pf p))).
+  Proof. trivial. Qed.
+
+  Global Instance normalform__Pair A B C D {nf__AC : Normalform A C} {nf__BD : Normalform B D} : Normalform (Pair A B) (Pair C D) :=
+    {
+      nf := fun x => nf__Pair x;
+      nf_impure := nf_impure__Pair nf__AC nf__BD
+    }.
+
+End Pair.
+
+Section List.
+  Inductive List A :=
+  | Nil' : List A
+  | Cons' : Prog A -> Prog (List A) -> List A.
+
+  Arguments Nil' {_}.
+
+  Definition consM A (fx : Prog A) (fxs : Prog (List A)) : Prog (List A) :=
+    pure (Cons' fx fxs).
+
+  Definition nilM {A} : Prog (List A) := pure (@Nil' A).
+
+  Definition headM A (fxs : Prog (List A)) : Prog A :=
+    fxs >>= fun xs => match xs with
+                   | Nil'      => @Fail A
+                   | Cons' x _ => x
+                   end.
+
+
+  Definition tailM A (fxs : Prog (List A)) : Prog (List A) :=
+    fxs >>= fun xs => match xs with
+                   | Nil'      => @Fail (List A)
+                   | Cons' _ xs => xs
+                   end.
+
+
+  Definition dupl A (fx : Prog A) : Prog (List A) :=
+    consM fx (consM fx (@nilM A)).
+
+  Definition duplShare A `{Shareable A} (fx : Prog A) : Prog (List A) :=
+    Share fx >>= fun x => consM x (consM x (@nilM A)).
+
+  Fixpoint appM' A (xs : List A) (fxs : Prog (List A)) : Prog (List A) :=
+    match xs with
+    | Nil'         => fxs
+    | Cons' fz fzs => consM fz (fzs >>= fun zs => appM' zs fxs)
+    end.
+
+  Definition appM A (fxs fys : Prog (List A)) : Prog (List A) :=
+    fxs >>= fun xs => appM' xs fys.
+
+  Definition shareArgs__List A `(Shareable A) `(Shareable (List A)) (xs : List A) : Prog (List A) :=
+    match xs with
+    | Nil'       => @nilM A
+    | Cons' y ys => Share y >>= fun sy => Share ys >>= fun sys => consM sy sys
+    end.
+
+  Global Instance shareable__List A `(sa : Shareable A) : Shareable (List A) :=
+    {
+      shareArgs := fun xs =>
+                     let fix aux xs :=
+                         let shr fp := Get >>= fun '(i,j) =>
+                                       Put (i + 1, j) >>= fun _ =>
+                                       pure (BeginShare (i,j) >>= fun _ =>
+                                             Put (i, j + 1) >>= fun _ =>
+                                             fp >>= fun x =>
+                                             aux x >>= fun x' =>
+                                             EndShare (i,j) >>= fun _ =>
+                                             pure x')
+                         in
+                         match xs with
+                         | Nil'       => @nilM A
+                         | Cons' y ys => Share y >>= fun sy => shr ys >>= fun sys => consM sy sys
+                         end
+                     in aux xs
+    }.
+
+  Fixpoint nf'__List A B `{Normalform A B} (xs : List A) : Prog (List B) :=
+    match xs with
+    | Nil'   => nilM
+    | Cons' sx sxs => nf sx >>= fun x =>
+                     sxs >>= fun xs =>
+                     nf'__List xs >>= fun xs' =>
+                     consM (pure x) (pure xs')
+    end.
+
+  Definition nf__List A B `{Normalform A B}  (stxs : Prog (List A)) : Prog (List B) :=
+    stxs >>= fun xs => nf'__List xs.
+
+ Lemma nf_impure__List A B nf__AB : forall s (pf : _ -> Prog (List A)),
+      @nf__List A B nf__AB (impure (ext s pf)) = impure (ext s (fun p => nf__List (pf p))).
+  Proof. trivial. Qed.
+
+  Global Instance normalform__List A B {nf__AB : Normalform A B} : Normalform (List A) (List B) :=
+    {
+      nf := fun x => nf__List x;
+      nf_impure := nf_impure__List nf__AB
+    }.
+
+  Fixpoint lengthM A (xs : List A) : Prog nat :=
+    match xs with
+    | Nil'        => pure 0
+    | Cons' _ fxs =>
+      let m := match fxs with
+               | pure xs => lengthM xs
+               | impure (ext (inl (sget _)) pf) =>
+                 pf (pget (42, 42)) >>= fun xs => lengthM xs
+               | impure (ext (inl (sput s'))   pf) =>
+                 pf (pput s') >>= fun xs => lengthM xs
+               | impure (ext (inr (inr sfail)) _)  => pure 0
+               | impure (ext (inr (inr (schoice mid))) pf) =>
+                 (pf true >>= fun xs => lengthM xs) >>= fun x =>
+                                                          (pf false >>= fun xs => lengthM xs) >>= fun y => pure (max x y)
+               | impure (ext (inr (inl (sbsharing n)))  pf) =>
+                 pf (pbsharing n) >>= fun xs => lengthM xs
+               | impure (ext (inr (inl (sesharing n)))  pf) =>
+                 pf (pesharing n) >>= fun xs => lengthM xs
+               end
+      in m >>= fun i => pure (i + 1)
+    end.
+
+  Fixpoint convert (xs : list nat) : Prog (List nat) :=
+    match xs with
+    | nil => nilM
+    | cons x xs => consM (pure x) (convert xs)
+    end.
+End List.
