Coq/src/HigherOrder/Free.v
@@ -7,45 +7,44 @@ Section Free.
 
   Inductive Free (C : HContainer H) A :=
   | pure : A -> Free C A
-  | impure : Ext Shape Pos Ctx (Free C) A -> Free C A.
+  | impure : Ext Shape Pos PosX Ctx (Free C) A -> Free C A.
 
 End Free.
 
 Arguments pure {_ _ _} _.
 
-(* Section Free_Rect. *)
+Section Free_Rect.
 
-(*   Variable H : (Type -> Type) -> Type -> Type. *)
-(*   Variable C__H : HContainer H. *)
-(*   Variable F : Type -> Type. *)
-(*   Variable A : Type. *)
-(*   Variable P : Free C__H A -> Type. *)
+  Variable H : (Type -> Type) -> Type -> Type.
+  Variable C__H : HContainer H.
+  Variable A : Type.
+  Variable P : Free C__H A -> Type.
 
-(*   Variable Pure_rect : forall (x : A), P (pure x). *)
-(*   Variable Impure_rect : forall (s : Shape) (pf : Pos s -> Free C__H A), *)
-(*       (forall p, P (pf p)) -> P (impure (ext s pf)). *)
+  Variable Pure_rect : forall (x : A), P (pure x).
+  Variable Impure_rect : forall (s : Shape) (pf : Pos s -> Free C__H A) pfx,
+      (forall p, P (pf p)) -> P (impure (ext s pf pfx)).
 
-(*   Fixpoint Free_Rect (fx : Free C__F A) : P fx := *)
-(*     match fx with *)
-(*     | pure x => Pure_rect x *)
-(*     | impure (ext s pf) => *)
-(*       Impure_rect s pf (fun p : Pos s => Free_Rect (pf p)) *)
-(*     end. *)
+  Fixpoint Free_Rect (fx : Free C__H A) : P fx :=
+    match fx with
+    | pure x => Pure_rect x
+    | impure (ext s pf pfx) =>
+      Impure_rect s pf pfx (fun p : Pos s => Free_Rect (pf p))
+    end.
 
-(* End Free_Rect. *)
+End Free_Rect.
 
-(* Section Free_Ind. *)
+Section Free_Ind.
 
-(*   Variable F : Type -> Type. *)
-(*   Variable C__F : Container F. *)
-(*   Variable A : Type. *)
-(*   Variable P : Free C__F A -> Prop. *)
+  Variable H : (Type -> Type) -> Type -> Type.
+  Variable C__H : HContainer H.
+  Variable A : Type.
+  Variable P : Free C__H A -> Prop.
 
-(*   Variable Pure_ind : forall (x : A), P (pure x). *)
-(*   Variable Impure_ind : forall (s : Shape) (pf : Pos s -> Free C__F A), *)
-(*       (forall p, P (pf p)) -> P (impure (ext s pf)). *)
+  Variable Pure_ind : forall (x : A), P (pure x).
+  Variable Impure_ind : forall (s : Shape) (pf : Pos s -> Free C__H A) pfx,
+      (forall p, P (pf p)) -> P (impure (ext s pf pfx)).
 
-(*   Definition Free_Ind (fx : Free C__F A) : P fx := Free_Rect P Pure_ind Impure_ind fx. *)
+  Definition Free_Ind (fx : Free C__H A) : P fx := Free_Rect P Pure_ind Impure_ind fx.
 
-(* End Free_Ind. *)
+End Free_Ind.
 
