Coq/src/HigherOrder/Prog.v
@@ -1,0 +1,13 @@
+Require Import Thesis.HigherOrder.Free.
+Require Import Thesis.HigherOrder.Container.
+
+Export Thesis.HigherOrder.Free.
+Export Thesis.HigherOrder.Container.
+
+Definition NDShare := C__Comb (C__State (nat * nat)) (C__Comb C__Sharing C__Choice).
+
+Definition NDShare__SC := C__Comb C__Sharing C__Choice.
+
+Definition Prog := Free NDShare.
+
+Definition Prog__SC := Free NDShare__SC.
